feat: Aig node constructors with proofs of basic invariants

Valaig/Aig/Basic.lean
@@ -1,4 +1,6 @@
-import Std.Sat.AIG
+import Std.Sat.AIG.Basic
+import Std.Sat.AIG.CachedGates
+import Valaig.Aig.StdSatLemmas
 
 namespace Valaig
 namespace Aig
@@ -24,6 +26,10 @@ def offset (v : Var) (n : Nat) : Var :=
 @[inline]
 def next (v : Var) : Var :=
   v.offset 1
+
+@[inline, simp, grind .]
+def ofRef {α} [DecidableEq α] [Hashable α] {aig : Std.Sat.AIG α} (ref : aig.Ref) : Var :=
+  .ofIdx ref.gate
 
 end Var
 
@@ -86,7 +92,11 @@ attribute [coe] ofFanin
 
 @[inline]
 def ofRef {α} [DecidableEq α] [Hashable α] {aig : Std.Sat.AIG α} (ref : aig.Ref) : Lit :=
-  .mk (.ofIdx ref.gate) ref.invert
+  .mk (.ofRef ref) ref.invert
+
+@[inline]
+def toRef {α} [DecidableEq α] [Hashable α] {aig : Std.Sat.AIG α} (lit : Lit) (h : lit.var.idx < aig.decls.size) : aig.Ref :=
+  .mk lit.var.idx lit.inverted h
 
 end Lit
 
@@ -111,9 +121,13 @@ deriving Hashable, DecidableEq, Repr, Inhabited
 
 namespace Input
 
-@[inline]
-def idx (input : Input) :=
+@[inline, reducible]
+def idx (input : Input) : Nat :=
   input.var.idx
+
+@[inline]
+def lit (input : Input) : Lit :=
+  input.var.toLit
 
 end Input
 
@@ -122,16 +136,20 @@ The metadata of a latch in the Aig
 -/
 structure Latch where
   var : Var
-  next : Lit
-  reset : Lit
+  next : Option Lit
+  reset : Option Lit := none
   symbol : String := ""
 deriving Hashable, DecidableEq, Repr, Inhabited
 
 namespace Latch
 
-@[inline]
-def idx (latch : Latch) :=
+@[inline, reducible]
+def idx (latch : Latch) : Nat :=
   latch.var.idx
+
+@[inline]
+def lit (latch : Latch) : Lit :=
+  latch.var.toLit
 
 end Latch
 
@@ -140,8 +158,8 @@ An atom in the combinational aig is either an input or a latch, which is just
 a reference back to the index in the inputs or latches arrays
 -/
 inductive Atom where
-| input : Nat -> Atom
-| latch : Nat -> Atom
+| input (idx : Nat) : Atom
+| latch (idx : Nat) : Atom
 deriving Hashable, DecidableEq, Repr, Inhabited
 
 /--
@@ -152,6 +170,43 @@ structure Output where
   lit : Lit
   symbol : String := ""
 deriving Hashable, DecidableEq, Repr, Inhabited
+
+abbrev Inputs := Array Input
+abbrev Latches := Array Latch
+abbrev Outputs := Array Output
+
+section
+variable {α : Type} {arr : Array α} {aig : Std.Sat.AIG Atom}
+
+@[simp]
+abbrev AtomInjec (idx : α -> Nat) (atom : Nat -> Atom) : Prop :=
+  ∀ (iarr : Nat) (harrbound : iarr < arr.size),
+  ∃ (hdeclbound : idx arr[iarr] < aig.decls.size),
+    aig.decls[idx arr[iarr]] = .atom (atom iarr)
+
+@[simp]
+abbrev AtomSurjec (idx : α -> Nat) (atom : Nat -> Atom) : Prop :=
+  ∀ (idecl : Nat) {iarr } (hdeclbound : idecl < aig.decls.size)
+    (hdecl : aig.decls[idecl] = .atom (atom iarr)),
+  ∃ (harrbound : iarr < arr.size),
+    idx arr[iarr] = idecl
+
+@[grind]
+structure AtomBijec (arr : Array α) (idx : α -> Nat) (aig : Std.Sat.AIG Atom) (atom : Nat -> Atom) : Prop where
+  hinjec : AtomInjec (arr := arr) (aig := aig) idx atom
+  hsurjec : AtomSurjec (arr := arr) (aig := aig) idx atom
+
+attribute [simp] AtomBijec.mk
+
+@[simp]
+abbrev InputBijec (arr : Inputs) (aig : Std.Sat.AIG Atom) : Prop :=
+  AtomBijec arr (·.idx) aig (.input ·)
+
+@[simp]
+abbrev LatchBijec (arr : Latches) (aig : Std.Sat.AIG Atom) : Prop :=
+  AtomBijec arr (·.idx) aig (.latch ·)
+
+end
 
 end Aig
 
@@ -166,44 +221,24 @@ structure Aig where
   aig : Std.Sat.AIG Aig.Atom
 
   -- A mapping from input indices (Atom.input idx) to their definition
-  inputs : Array Aig.Input
+  inputs : Aig.Inputs
 
   -- A mapping from latch indices (Atom.latch idx) to their definition
-  latches : Array Aig.Latch
+  latches : Aig.Latches
 
   -- A set of literals that should never be true
-  bads : Array Aig.Output
+  bads : Aig.Outputs
 
   -- Only index 0 represents false
-  hfalse : ∀ {i} (h : i < aig.decls.size), aig.decls[i] = .false ↔ i = 0
+  hfalse : ∀ (i : Nat) (h : i < aig.decls.size), aig.decls[i] = .false ↔ i = 0
 
-  -- Input indices map to corresponding atoms
-  hinputstodecl :
-    ∀ {iin idecl} (hin : iin < inputs.size)
-      (_ : inputs[iin].idx = idecl),
-    ∃ (hdecl : idecl < aig.decls.size),
-      aig.decls[idecl] = .atom (.input iin)
+  -- There is a bijection between indices in the inputs array and input atoms
+  -- in the aig
+  hinputmap : Aig.InputBijec inputs aig
 
-  -- Input atoms map to corresponding indices
-  hdecltoinputs :
-    ∀ {iin idecl} (hdecl : idecl < aig.decls.size)
-      (_ : aig.decls[idecl] = .atom (.input iin)),
-    ∃ (hin : iin < inputs.size),
-      inputs[iin].idx = idecl
-
-  -- Latch indices map to corresponding atoms
-  hlatchestodecl :
-    ∀ {ilat idecl} (hlat : ilat < latches.size)
-      (_ : latches[ilat].idx = idecl),
-    ∃ (hdecl : idecl < aig.decls.size),
-      aig.decls[idecl] = .atom (.latch ilat)
-
-  -- Latch atoms map to corresponding indices
-  hdecltolatches :
-    ∀ {ilat idecl} (hdecl : idecl < aig.decls.size)
-      (_ : aig.decls[idecl] = .atom (.latch ilat)),
-    ∃ (hlat : ilat < latches.size),
-      latches[ilat].idx = idecl
+  -- There is a bijection between indices in the latches array and latch atoms
+  -- in the aig
+  hlatchmap : Aig.LatchBijec latches aig
 
   -- Resets are stratified. TODO: This definition doesn't work as the binary
   -- aiger format requires latches come before gates, so you can't define
@@ -213,19 +248,36 @@ structure Aig where
   -- way easier)
   -- hreset : ∀ {latch}, latch ∈ latches → latch.reset.var < latch.var
 
+structure Aig.WF (aig : Aig) where
+  -- We specify that each latch must have a next state as an external
+  -- well-formedness predicate as
+  hnext : ∀ {latch}, latch ∈ aig.latches → latch.next.isSome
+
+  -- TODO: Should other predicates be here too? There are other cases when it
+  -- could be nice to be able to momentarily break invariants, in particular
+  -- hreset
+
+-- Allow grind to get at the Aig invariants
+attribute [grind =] Aig.aig
+attribute [grind! .] Std.Sat.AIG.hzero
+attribute [grind! .] Std.Sat.AIG.hconst
+attribute [grind =] Aig.hfalse
+attribute [grind! .] Aig.hinputmap
+attribute [grind! .] Aig.hlatchmap
+
 namespace Aig
 
 @[inline]
 def size (aig : Aig) : Nat := aig.aig.decls.size
 
 @[inline]
-def numConstants (_ : Aig) : Nat := 1
+abbrev numConstants (_ : Aig) : Nat := 1
 
 @[inline]
-def numInputs (aig : Aig) : Nat := aig.inputs.size
+abbrev numInputs (aig : Aig) : Nat := aig.inputs.size
 
 @[inline]
-def numLatches (aig : Aig) : Nat := aig.latches.size
+abbrev numLatches (aig : Aig) : Nat := aig.latches.size
 
 -- Number of inputs and latches
 @[inline]
@@ -239,10 +291,124 @@ def numLeaves (aig : Aig) : Nat := aig.numAtoms + aig.numConstants
 def numGates (aig : Aig) : Nat := aig.size - aig.numLeaves
 
 @[inline]
-def numBads (aig : Aig) : Nat := aig.bads.size
+abbrev numBads (aig : Aig) : Nat := aig.bads.size
 
 @[inline]
 def maxVar (aig : Aig) : Var := .ofIdx (aig.size - 1)
+
+@[inline]
+abbrev Lit.validIn (lit : Lit) (aig : Aig) := lit.var.idx < aig.size
+
+@[inline]
+def empty : Aig :=
+  {
+    aig := .empty
+    inputs := #[],
+    latches := #[],
+    bads := #[],
+    hfalse := by simp [Std.Sat.AIG.empty],
+    hinputmap := by simp [Std.Sat.AIG.empty],
+    hlatchmap := by simp [Std.Sat.AIG.empty],
+  }
+
+@[inline]
+abbrev nextInputIdx (aig : Aig) : Nat :=
+  aig.numInputs
+
+@[inline]
+abbrev nextLatchIdx (aig : Aig) : Nat :=
+  aig.numLatches
+
+theorem nextInputIdx_notIn_decls {aig : Aig} {i : Nat} (h : i < aig.size) :
+    aig.aig.decls[i] ≠ .atom (.input aig.nextInputIdx) := by
+  have := aig.hinputmap.hsurjec i (iarr := aig.nextInputIdx) h
+  grind
+
+theorem nextLatchIdx_notIn_decls {aig : Aig} {i : Nat} (h : i < aig.size) :
+    aig.aig.decls[i] ≠ .atom (.latch aig.nextLatchIdx) := by
+  have := aig.hlatchmap.hsurjec i (iarr := aig.nextLatchIdx) h
+  grind
+
+@[inline]
+def addInput (aig : Aig) (symbol : String := "") : Aig × Lit :=
+  -- We don't need to use mkAtomCached as nextInputIdx_notIn_decls guarantees
+  -- it would be a miss
+  let res := aig.aig.mkAtom <| .input aig.nextInputIdx
+  let input := { var := .ofRef res.ref, symbol }
+
+  let aig := { aig with
+    aig := res.aig,
+    inputs := aig.inputs.push input,
+    hfalse := by grind,
+    hinputmap := by grind,
+    hlatchmap := by grind,
+  }
+  (aig, input.lit)
+
+@[inline]
+def addGate (aig : Aig) (rhs0 rhs1 : Lit) {h0 : rhs0.validIn aig} {h1 : rhs1.validIn aig} :
+    Aig × Lit :=
+  let res := aig.aig.mkAndCached ⟨rhs0.toRef h0, rhs1.toRef h1⟩
+
+  let aig := { aig with
+    aig := res.aig,
+    hfalse := by
+      intro i
+      by_cases i < aig.aig.decls.size
+      · grind
+      · -- For some reason if I remove this grind hits an error
+        have : i ≠ 0 := by grind only [Std.Sat.AIG.hzero]
+        grind,
+    hinputmap := by grind
+    hlatchmap := by grind
+  }
+  (aig, Lit.ofRef res.ref)
+
+@[inline]
+def addLatch (aig : Aig) (next : Lit) (reset : Option Lit := none) (symbol : String := "") : Aig × Lit :=
+  -- We don't need to use mkAtomCached as nextLatchIdx_notIn_decls guarantees
+  -- it would be a miss
+  let res := aig.aig.mkAtom <| .latch aig.nextLatchIdx
+  let latch := {
+    var := .ofRef res.ref,
+    next,
+    reset,
+    symbol
+  }
+
+  let aig := { aig with
+    aig := res.aig,
+    latches := aig.latches.push latch,
+    hfalse := by grind,
+    hinputmap := by grind,
+    hlatchmap := by grind,
+  }
+  (aig, latch.lit)
+
+@[inline]
+def addLatch' (aig : Aig) (reset : Option Lit := none) (symbol : String := "") : Aig × Lit :=
+  -- We don't need to use mkAtomCached as nextLatchIdx_notIn_decls guarantees
+  -- it would be a miss
+  let res := aig.aig.mkAtom <| .latch aig.nextLatchIdx
+  let latch := {
+    var := .ofRef res.ref,
+    next := none,
+    reset,
+    symbol
+  }
+
+  let aig := { aig with
+    aig := res.aig,
+    latches := aig.latches.push latch,
+    hfalse := by grind,
+    hinputmap := by grind,
+    hlatchmap := by grind,
+  }
+  (aig, latch.lit)
+
+@[inline]
+def addBad (aig : Aig) (lit : Lit) (symbol : String := "") : Aig :=
+  { aig with bads := aig.bads.push { lit, symbol } }
 
 -- [>-
 -- A timeframe in the execution of the model, starting from the initial state at 0
