Valaig/Aig/StdSatLemmas.lean
@@ -1,0 +1,54 @@
+import Std.Sat.AIG.Basic
+import Std.Sat.AIG.Cached
+import Std.Sat.AIG.CachedGates
+import Std.Sat.AIG.CachedLemmas
+import Std.Sat.AIG.CachedGatesLemmas
+
+namespace Valaig.Aig
+
+open Std.Sat AIG
+
+variable {α : Type} [Hashable α] [DecidableEq α]
+
+/--
+`AIG.mkAtom` only appends a single atom to the underlying AIG.
+-/
+@[simp, grind! .]
+theorem mkAtom_eq_decl_push (aig : AIG α) (var : α) :
+    (aig.mkAtom var).aig.decls = aig.decls.push (.atom var) := by
+  simp [mkAtom]
+
+/--
+`AIG.mkAtom` returns a reference to the next element in the underlying AIG
+-/
+@[simp, grind! .]
+theorem mkAtom_ref_eq_decl_size (aig : AIG α) (var : α) :
+    (aig.mkAtom var).ref.gate = aig.decls.size := by
+  simp [mkAtom]
+
+/--
+- `AIG.mkGateCached` only potentially appends gates, not atoms/constants
+-/
+@[simp, grind! .]
+theorem mkGateCached_matches_gate (idx : Nat) (aig : AIG α) (input : aig.BinaryInput)
+    {hlow : idx ≥ aig.decls.size} {hhigh : idx < (aig.mkGateCached input).aig.decls.size} :
+    (aig.mkGateCached input).aig.decls[idx] matches .gate _ _ := by
+  simp only [mkGateCached, mkGateCached.go]
+  grind
+
+attribute [simp, grind! .] mkGateCached_decl_eq
+attribute [simp, grind! .] mkGateCached_le_size
+
+/--
+- `AIG.mkAndCached` only potentially appends gates, not atoms/constants
+-/
+@[simp, grind! .]
+theorem mkAndCached_matches_gate (idx : Nat) (aig : AIG α) (input : aig.BinaryInput)
+    {hlow : idx ≥ aig.decls.size} {hhigh : idx < (aig.mkAndCached input).aig.decls.size} :
+    (aig.mkAndCached input).aig.decls[idx] matches .gate _ _ := by
+  simp_all [mkAndCached]
+
+attribute [simp, grind! .] mkAndCached_decl_eq
+attribute [simp, grind! .] mkAndCached_le_size
+
+end Valaig.Aig
